imper/Swap.ml
@@ -4,13 +4,3 @@ let swap i j =
    i := !j;
    j := t
 
-
-(* another test about aliasing *)
-
-let alias () =
-   let x = ref 1 in
-   let a = ref x in
-   let y = !a in
-   let b = ref y in
-   incr (!b);
-   (!a, a)
