vacid/union_find_compo.ml
@@ -1,0 +1,34 @@
+
+type state = {
+   mutable nb_compo : int;
+   mutable parent : int array; }
+
+let create size =
+   { nb_compo = size;
+     parent = Array.init size (fun i -> i) }
+
+let get_nb_compo s =
+   s.nb_compo
+
+let rec find s a =
+   if s.parent.(a) = a 
+      then a   
+      else find s s.parent.(a)
+
+let union s a b =
+   let ra = find s a in
+   let rb = find s b in
+   if ra <> rb then begin
+      s.parent.(ra) <- rb;
+      s.nb_compo <- s.nb_compo - 1;
+   end
+
+let same_compo s a b =
+   find s a = find s b
+
+
+(*
+let build_maze n =
+   let s = create (n*n) in
+   while get_nb_compo s > 1 do
+*) 
