vacid/union_find_proof.v
@@ -1,59 +1,222 @@
+Set Implicit Arguments.
+Require Import CFLib LibSet LibMap LibArray sparse_array_ml.
 
 
-Definition partition A := set (set A).
+(****************************************************)
+(** Shorthand *)
+
+Notation "'tab'" := (array int).
+Notation "'L'" := maxlen.
+
+Definition SarrayPacked :=
+  @Sarray int (array int) (array int) (array int) Id (Array Id) (Array Id) (Array Id).
+
+Definition SarrayUnpacked :=
+  @Sarray int loc loc loc Id Id Id Id.
+
+
+(****************************************************)
+(** Invariant *)
+
+(** [good_sizes] asserts that the three arrays have size [L] *)
+
+Definition good_sizes n (Val Idx Back : tab) :=
+  length Val = L /\ length Idx = L /\ length Back = L /\ 0 <= n <= L.
+
+(** [i] is a [Valid] index if [Back(k) = i] for some [k] *)
+
+Definition Valid n (Idx Back : tab) i :=
+  index L i /\ let k := Idx\(i) in 
+  index n k /\ Back\(k) = i.
+
+(** [BackCorrect] holds when [k < n -> Idx(Back(k)) = k]*)
+
+Definition BackCorrect n (Idx Back:tab) :=
+  forall k, index n k ->
+  let i := Back\(k) in index L i /\ Idx\(i) = k.
+
+(** [s ~> SparseArray f] indicates that [s] is a record 
+    describing a sparse array whose model is the function [f] *)
+
+Definition SparseArray (f:int->int) (s:loc) :=
+  Hexists (n:int) (Val:tab) (Idx:tab) (Back:tab),
+     s ~> SarrayPacked n Val Idx Back
+  \* [ good_sizes n Val Idx Back
+       /\ BackCorrect n Idx Back
+       /\ (forall i, f i = If Valid n Idx Back i then Val\(i) else 0) ].
+
+
+(****************************************************)
+(** Automation *)
+
+(** Automation of [index] goals *)
+
+Ltac myunfold := 
+  repeat match goal with 
+  | H: Valid _ _ _ _ |- _ => hnf in H 
+  | H: good_sizes _ _ _ _ |- _ => hnf in H 
+  end; jauto_set.
+
+Hint Extern 1 (@index _ _ (array_index _) ?t ?i) =>
+  myunfold; eassumption.
+Hint Extern 1 (@index _ _ int_index ?t ?i) =>
+  myunfold; eassumption.
+Hint Extern 1 (@index _ _ (array_index _) ?t ?i) =>
+  myunfold; match goal with H: @index _ _ int_index ?n i |- _ => 
+    eapply index_array_length end.
+
+Lemma index_array_length_le : forall A (t : array A) n i,
+  index n i -> n <= length t -> index t i.
+Proof.
+  intros. subst. rewrite array_index_def.
+  rewrite @int_index_def in *. math.
+Qed.
+
+Ltac strong := 
+  math_0; math_1; math_2; math_3; try split; 
+  eapply int_index_prove; math_3; math_4; math_5.
+
+(** Tactic for rewriting *)
+
+Tactic Notation "inhabs" := (* workaround coq bug *)
+  try match goal with |- Inhab _ => typeclass end.
+Tactic Notation "rew_map_array" :=
+  rew_map; rew_array; inhabs.
+Tactic Notation "rew_map_array" "~" :=
+  rew_map_array; auto~; inhabs.
+Tactic Notation "rew_map_array" "*" :=
+  rew_map_array; auto*; inhabs.
+
+
+(****************************************************)
+(** Verification *)
+
+(*--------------------------------------------------*)
+(** Function [valid] *)
+
+Lemma valid_spec :
+  Spec valid i s |R>> forall n Val Idx Back, 
+    good_sizes n Val Idx Back -> index L i -> n <= L ->
+    keep R (s ~> SarrayPacked n Val Idx Back)
+           (\= istrue (Valid n Idx Back i)).
+Proof.
+  xcf. introv Siz Ii Le. unfold SarrayPacked.
+  xchange (Sarray_focus s) as n' val idx back E. subst n'.
+  xapps. xapps*. xapps. xif. 
+  (* case inbound *)
+  xapps. xapps. hnf in Siz. eapply array_index_prove. math.
+  xchange (Sarray_unfocus s).
+  xret. hsimpl. rew_logics. unfolds Valid. splits*.
+  (* case outof bound *)
+  xchange (Sarray_unfocus s). 
+  xret. hsimpl. fold_bool. fold_prop. unfold Valid.
+  cuts*: (~ index n (Idx\(i))). rewrite* int_index_def.
+Qed.
+
+Hint Extern 1 (RegisterSpec valid) => Provide valid_spec.
+
+
+(*--------------------------------------------------*)
+(** Function [get] *)
+
+Lemma get_spec' :
+  Spec get i s |R>> forall f, index L i -> 
+    keep R (s ~> SparseArray f) (\= f i).
+Proof.
+  xcf. introv ILi.
+  unfold SparseArray. hdata_simpl.
+  xextract as n Val Idx Back (Siz&Bok&Iok).
+  xapps*. hnf in Siz; math.
+  lets M: Iok i. xif; case_if in M; tryfalse.
+  (* case is an index *)
+  xchange (Sarray_focus s) as n' val idx back E. subst n'. xapps. xapp*.
+  intros r. hchanges (Sarray_unfocus s); subst~.
+  (* case not an index *)
+  xrets*.
+Qed. 
+
+
+(*--------------------------------------------------*)
+(** Function [set] *)
+
+(** Auxiliary definition for update of a function *)
+
+Definition update_fun A B (f:A->B) i v :=
+  fun j => If i '= j then v else f j.
+
+(** Auxiliary lemma for back pointers *)
+
+Lemma not_Valid_to_notin_Back : forall i n Idx Back,
+  ~ (Valid n Idx Back i) -> index L i -> BackCorrect n Idx Back ->
+  (forall k, index n k -> i <> Back\(k)).
+Proof.
+  introv NVi ILi Bok Ink Eq. forwards~ [_ E]: Bok k. 
+  unfolds Valid. rewrite (prop_eq_True_back ILi) in NVi. 
+  rew_logic in NVi. destruct NVi as [H|H]; apply H; clear H; congruence.
+Qed.
+
+(** Auxiliary lemma for validity of indices *)
+
+Lemma Valid_extend : forall n Idx Back i j,
+  length Idx = L -> length Back = L -> index L n -> i <> j ->
+  (Valid n Idx Back j <-> Valid (n + 1) (Idx\(i:=n)) (Back\(n:=i)) j).
+Proof.
+  introv Le1 Le2 ILn Neq. unfold Valid. 
+  lets M: ILn. rewrite int_index_def in M.
+  test_prop (index L j); [|auto*].
+  rewrite~ (array_update_read_neq (t:=Idx)).
+  rewrite int_index_succ; [|math].
+  test_prop (index n (Idx\(j))).
+    rew_array*.                           (* easy for SMT *)
+      apply* index_array_length_le. math. (* easy for SMT *)
+      rewrite int_index_def in *. math.   (* easy for SMT *)
+    split; auto_false. intros [In Eq].    (* easy for SMT *)
+     rewrite In in Eq.                    (* easy for SMT *)
+     rewrite array_update_read_eq in Eq; auto_false. (* easy for SMT *)
+Qed.
+
+(** Verification of the [set] function *)
+
+Lemma set_spec :
+  Spec set i v l |R>> forall f, index L i ->
+    R (l ~> SparseArray f) (# l ~> SparseArray (update_fun f i v)).
+Proof.
+  xcf. introv Imi. hdata_simpl SparseArray.
+  xextract as n Val Idx Back (Siz&Bok&Iok).
+  xchange (Sarray_focus s) as n' val idx back. intro_subst.
+  xapps. xapps*.
+  xchange (Sarray_unfocus s n). fold SarrayPacked. clear val idx back.
+  xapps*. hnf in Siz; math. xif.
+  (* case create back-index *)
+  xchange (Sarray_focus s) as n' val idx back. intro_subst.
+  lets Nbk: not_Valid_to_notin_Back Bok; eauto.
+  skip: (n < L). (* pigeon-holes, see task description *)
+  asserts: (0 <= n < L). hnf in Siz; math.                 (* easy for SMT *)
+  asserts: (index L n). rewrite~ int_index_def.            (* easy for SMT *)
+  xapps. xapps. xapps*. xapps. xapps*. xapp.
+  hchanges (Sarray_unfocus s). splits.
+    hnf. rew_array. hnf in Siz. jauto_set; auto; math.     (* easy for SMT *)
+    intros k Ik. tests (k = n).                            (* easy for SMT *)
+      rew_array*.                                          (* easy for SMT *)
+      rewrite @int_index_def in Ik.                        (* easy for SMT *)
+       asserts [? ?]: (index n k /\ index L k). strong.    (* easy for SMT *)
+       forwards~ [? ?]: Bok k. rew_array*.                 (* easy for SMT *)
+    intros j. unfold update_fun. specializes Iok j. case_if.
+      asserts: (index (n + 1) n).                          (* easy for SMT *)
+        eapply int_index_prove; math.                      (* easy for SMT *)
+       subst. unfold Valid. rew_map_array*.                (* easy for SMT *)
+       case_if; tryfalse*; auto.                           (* easy for SMT *)
+      rewrite Iok. apply~ If_eq.
+        myunfold. apply~ Valid_extend.
+        intros. rew_array~.                                (* easy for SMT *)
+  (* case nothing to do *)
+   xret. hsimpl. splits~. unfold update_fun.
+   intros j. specializes Iok j.                            (* easy for SMT *)
+   case_if; case_if; tryfalse; auto.                       (* easy for SMT *)
+     subst. rew_map_array*.                                (* easy for SMT *)
+     rew_map_array*.                                       (* easy for SMT *)
+Qed.
 
 
 
-Definition union_find_graph (Parent : int array) (G : sgraph int) :=
-     nodes G = range 0 (size Parent - 1)
-  /\ forest (transpose G)
-  /\ forall_ x \in nodes G, Parent\[x] \in nodes G
-                         /\ outgoing G x = Parent\[x].
 
-     (* edges G = \{ (x,Parent\[x]) | x \in nodes G } *)
-
-
-Definition Struct (P:partition int) (l:loc) :=
-  hexists nb_compo parent Parent G,
-    l ~> state_of nb_compo parent
-  * parent ~> Array Pure Parent
-  * [ union_find_graph Parent G ]
-  * [ P = equiv_classes (unweighed_of G) ]
-  * [ nb_compo = card P ].
-
-
-Definition full_partition (E:set A) :=
-  (* returns {{x1},{x2},..,{xn}} when
-     E is {x1,x2,..xn} *) .
-
-Definition partition_item (P:set (set A)) (x:A) :=
-  exists_ E \in P, x \in E.
-
-Definition partition_merge P x y :=
-  (* returns a new partition where the set containing x
-     has been merged with the set containing y *) 
-
-Definition partition_same P x y :=
-  exists_ E \in P /\ x \in E /\ y \in E.
-
-Lemma create_spec :
-  Spec create n |R>> n >= 0 ->
-    R [] (_~> Struct (full_partition (range 0 (n-1)))).
-
-Lemma union_spec : 
-  Spec union s a b |R>> forall P,
-    partition_item P a -> partition_item P b ->
-    R (s ~> Struct P) (s ~> Struct (partition_merge P a b)).
-    
-Lemma same_compo_spec :
-  Spec same_compo s a b |R>> forall P,
-    partition_item P a -> partition_item P b ->
-    keep R (s ~> Struct P) (bool_of (partition_same P a b)). 
-
-
-(* variante:
-Lemma union_spec : 
-  Spec union s a b |R>> forall E P,
-    a \in E -> b \in E -> partition_of E P ->
-    R (s ~> Struct P) (s ~> Struct (partition_merge P a b)).
-*)
